\centerline{Steve Hsu\hfill workshop 3}
Let $a_n = \root n \of n - 1$.
We will first show that $(a_n) \to 0$.
We have $n = (1 + a_n)^n = \sum _{k = 0} ^n {n \choose k} a_n^k \ge
{n \choose 2} a_n^2$.
Simplifying the inequality, $a_n \le \sqrt {2 \over n - 1}$.
Since $\root n \of n \ge 1$ for all natural numbers $n$,
we have $0 \le a_n \le \sqrt {2 \over n - 1}$.
Since $(\sqrt {2 \over n - 1}) \to 0$, by the squeeze theorem,
$(a_n) \to 0$.
Since $(1) \to 1$, by the algebraic limit theorem,
$(\root n \of n) \to 1$.
\bye
