\centerline{Steve Hsu\hfill workshop 4}
\item{a.}

Given a real number $M$, take $N$ such that
for every $n \ge N$, $b_n > M - a + 1$ and $a_n > a - 1$.
Then for $n \ge N$, $a_n + b_n > M - a + 1 + a - 1 = M$, as desired.
\bigskip
\item{b.}

Let $a_n = c - n$ and $b_n = n$ for every natural number $n$.
Given a real number $M$, take $N > c - M$.
Then for $n \ge N$, $a_n = c - n \le c - N < M$, so $(a_n) \to -\infty$.
Given a real number $M$, take $N > M$.
Then for $n \ge N$, $b_n = n \ge N > M$, so $(b_n) \to +\infty$.
Notice that $a_n + b_n = c$ for every natural number $n$,
so $(a_n + b_n) \to c$.

Let $a_n = -n$ and $b_n = 2n$ for every natural number $n$.
Clearly, $(a_n) \to -\infty$ and $(b_n) \to +\infty$.
Since $a_n + b_n = n$ for each natural number $n$,
$(a_n + b_n) \to +\infty$.

Similarly, let $a_n = -2n$ and $b_n = n$ for every natural number $n$.
Then $(a_n) \to -\infty$, $(b_n) \to +\infty$, and $(a_n + b_n) \to -\infty$.
\bye
